Lean4Nbe/Typed_Lambda_Norm.lean
@@ -1,0 +1,34 @@
+/-
+data Type = NAT | FUN Type Type
+
+data Term = Var Integer | App Term Term | Lam Type Term
+| Zero | Succ Term | Rec Type Term Term Term
+
+mutual begin
+data No = Lam Type No | Zero | Succ No | Ne Ne
+
+data Ne = Var Integer | App Ne No | Rec Type No No Ne
+mutual end
+
+data D = LamD Type (D -> D) -- semantic function
+| ZeroD -- normal 0
+| SuccD D -- normal successor
+| NeD TERM -- neutral term family
+
+Term families
+type TERM = Integer -> Term
+
+reify :: D -> TERM
+reify (LamD a f) k
+    = Lam a (reify (f (reflect a (freevar (-(k+1))))) (k+1))
+reify ZeroD k = Zero
+reify (SuccD d) k = Succ (reify d k)
+reify (NeD t) k = t k
+
+reflect :: Type -> TERM -> D
+reflect (FUN a b) t
+    = LamD a (\d -> reflect b (app t (reify d)))
+reflect NAT t = NeD t
+
+
+-/
