lakefile.lean
@@ -11,6 +11,9 @@ package «lean4-nbe» where
 require mathlib from git
   "https://github.com/leanprover-community/mathlib4.git"
 
+require verso from git
+  "https://github.com/leanprover/verso.git" @ "main"
+
 @[default_target]
 lean_lib «Lean4Nbe» where
   -- add any library configuration options here
